Adding methods to support :-, covariance on type parameters

src/Wrappers.dfy
@@ -8,35 +8,65 @@
 
 module Wrappers {
   
-  datatype Option<T> = None | Some(value: T) {
-    function method ToResult(): Result<T, string> 
-    {
+  datatype Option<+T> = None | Some(value: T) {
+    function method ToResult(): Result<T, string> {
       match this
       case Some(v) => Success(v)
       case None() => Failure("Option is None")
     }
     
-    function method UnwrapOr(default: T): T 
-    {
+    function method UnwrapOr(default: T): T {
       match this
       case Some(v) => v
       case None() => default
     }
+
+    predicate method IsFailure() {
+      None?
+    }
+
+    function method PropagateFailure<U>(): Option<U>
+      requires None?
+    {
+      None
+    }
+
+    function method Extract(): T
+      requires Some?
+    {
+      value
+    }
   }
-  
-  datatype Result<T, R> = | Success(value: T) | Failure(error: R) {
+
+  datatype Result<+T, +R> = | Success(value: T) | Failure(error: R) {
     function method ToOption(): Option<T> 
     {
       match this
       case Success(s) => Some(s)
       case Failure(e) => None()
     }
+
     function method UnwrapOr(default: T): T 
     {
       match this
       case Success(s) => s
       case Failure(e) => default
     }
+
+    predicate method IsFailure() {
+      Failure?
+    }
+
+    function method PropagateFailure<U>(): Result<U, R>
+      requires Failure?
+    {
+      Failure(this.error)
+    }
+
+    function method Extract(): T
+      requires Success?
+    {
+      value
+    }
   }
-  
 }
